Removed unnecessary return depths

06TreeCode/TreeCode.thy
@@ -5,7 +5,7 @@ begin
 datatype tree_code = 
   TLookup nat
   | TPushCon nat
-  | TPushLam "tree_code list" nat
+  | TPushLam "tree_code list"
   | TApply
 
 datatype tclosure = 
@@ -20,14 +20,14 @@ fun full_block :: "tree_code list \<Rightarrow> nat \<rightharpoonup> nat" where
   "full_block [] n = Some n"
 | "full_block (TLookup x # cd) n = full_block cd (Suc n)"
 | "full_block (TPushCon k # cd) n = full_block cd (Suc n)"
-| "full_block (TPushLam cd' d # cd) n = full_block cd (Suc n)"
+| "full_block (TPushLam cd' # cd) n = full_block cd (Suc n)"
 | "full_block (TApply # cd) 0 = None"
 | "full_block (TApply # cd) (Suc n) = full_block cd n"
 
 primrec full_code_closure :: "tree_code \<Rightarrow> bool" where
   "full_code_closure (TLookup x) = True"
 | "full_code_closure (TPushCon k) = True"
-| "full_code_closure (TPushLam cd d) = (full_block cd 0 = Some 1 \<and> list_all full_code_closure cd)"
+| "full_code_closure (TPushLam cd) = (full_block cd 0 = Some 1 \<and> list_all full_code_closure cd)"
 | "full_code_closure TApply = True"
 
 primrec full_closure :: "tclosure \<Rightarrow> bool" where
@@ -45,7 +45,7 @@ inductive evalt :: "tree_code_state \<Rightarrow> tree_code_state \<Rightarrow> 
   evt_lookup [simp]: "lookup env x = Some v \<Longrightarrow> 
     TS vs ((env, TLookup x # cd) # sfs) \<leadsto>\<^sub>t TS (v # vs) ((env, cd) # sfs)"
 | evt_pushcon [simp]: "TS vs ((env, TPushCon k # cd) # sfs) \<leadsto>\<^sub>t TS (TConst k # vs) ((env, cd) # sfs)"
-| evt_pushlam [simp]: "TS vs ((env, TPushLam cd' (length env) # cd) # sfs) \<leadsto>\<^sub>t 
+| evt_pushlam [simp]: "TS vs ((env, TPushLam cd' # cd) # sfs) \<leadsto>\<^sub>t 
     TS (TLam env cd' # vs) ((env, cd) # sfs)"
 | evt_apply [simp]: "TS (v # TLam env' cd' # vs) ((env, TApply # cd) # sfs) \<leadsto>\<^sub>t 
     TS vs ((v # env', cd') # (env, cd) # sfs)"
@@ -71,18 +71,14 @@ proof (induction \<Sigma> \<Sigma>' rule: evalt.induct)
     by (induction "TS vs ((env, TLookup x # cd) # sfs)" \<Sigma>'' rule: evalt.induct) simp_all 
 next
   case (evt_pushcon vs env k cd sfs)
-  thus ?case 
-    by (induction "TS vs ((env, TPushCon k # cd) # sfs)" \<Sigma>'' rule: evalt.induct) simp_all 
+  thus ?case by (induction "TS vs ((env, TPushCon k # cd) # sfs)" \<Sigma>'' rule: evalt.induct) simp_all 
 next
   case (evt_pushlam vs env cd' cd sfs)
-  thus ?case 
-    by (induction "TS vs ((env, TPushLam cd' (length env) # cd) # sfs)" \<Sigma>'' rule: evalt.induct) 
-       simp_all 
+  thus ?case by (induction "TS vs ((env, TPushLam cd' # cd) # sfs)" \<Sigma>'' rule: evalt.induct) simp_all 
 next
   case (evt_apply v env' cd' vs env cd sfs)
   thus ?case 
-    by (induction "TS (v # TLam env' cd' # vs) ((env, TApply # cd) # sfs)" \<Sigma>'' 
-        rule: evalt.induct) 
+    by (induction "TS (v # TLam env' cd' # vs) ((env, TApply # cd) # sfs)" \<Sigma>'' rule: evalt.induct) 
        simp_all 
 next
   case (evt_return vs env sfs)
