07TailCall/TailCall.thy
@@ -3,13 +3,13 @@ theory TailCall
 begin
 
 datatype tco_return =
-    TCOReturn nat
-  | TCOJump nat
+    TCOReturn
+  | TCOJump
 
 datatype tco_code = 
   TCOLookup nat
   | TCOPushCon nat
-  | TCOPushLam "tco_code list" tco_return nat
+  | TCOPushLam "tco_code list" tco_return
   | TCOApply
 
 datatype tco_closure = 
@@ -25,14 +25,13 @@ inductive evaltco :: "tco_code_state \<Rightarrow> tco_code_state \<Rightarrow> 
     TCOS vs ((env, TCOLookup x # cd, r) # sfs) \<leadsto>\<^sub>t\<^sub>c\<^sub>o TCOS (v # vs) ((env, cd, r) # sfs)"
 | evtco_pushcon [simp]: "TCOS vs ((env, TCOPushCon k # cd, r) # sfs) \<leadsto>\<^sub>t\<^sub>c\<^sub>o 
     TCOS (TCOConst k # vs) ((env, cd, r) # sfs)"
-| evtco_pushlam [simp]: "TCOS vs ((env, TCOPushLam cd' r' (length env) # cd, r) # sfs) \<leadsto>\<^sub>t\<^sub>c\<^sub>o 
+| evtco_pushlam [simp]: "TCOS vs ((env, TCOPushLam cd' r' # cd, r) # sfs) \<leadsto>\<^sub>t\<^sub>c\<^sub>o 
     TCOS (TCOLam env cd' r' # vs) ((env, cd, r) # sfs)"
 | evtco_apply [simp]: "TCOS (v # TCOLam env' cd' r' # vs) ((env, TCOApply # cd, r) # sfs) \<leadsto>\<^sub>t\<^sub>c\<^sub>o 
     TCOS vs ((v # env', cd', r') # (env, cd, r) # sfs)"
-| evtco_return [simp]: "TCOS vs ((env, [], TCOReturn (length env)) # sfs) \<leadsto>\<^sub>t\<^sub>c\<^sub>o TCOS vs sfs"
-| evtco_jump [simp]: 
-    "TCOS (v # TCOLam env' cd' r' # vs) ((env, [], TCOJump (length env)) # sfs) \<leadsto>\<^sub>t\<^sub>c\<^sub>o 
-      TCOS vs ((v # env', cd', r') # sfs)"
+| evtco_return [simp]: "TCOS vs ((env, [], TCOReturn) # sfs) \<leadsto>\<^sub>t\<^sub>c\<^sub>o TCOS vs sfs"
+| evtco_jump [simp]: "TCOS (v # TCOLam env' cd' r' # vs) ((env, [], TCOJump) # sfs) \<leadsto>\<^sub>t\<^sub>c\<^sub>o 
+    TCOS vs ((v # env', cd', r') # sfs)"
 
 theorem determinismt: "\<Sigma> \<leadsto>\<^sub>t\<^sub>c\<^sub>o \<Sigma>' \<Longrightarrow> \<Sigma> \<leadsto>\<^sub>t\<^sub>c\<^sub>o \<Sigma>'' \<Longrightarrow> \<Sigma>' = \<Sigma>''"
 proof (induction \<Sigma> \<Sigma>' rule: evaltco.induct)
@@ -46,8 +45,7 @@ next
 next
   case (evtco_pushlam vs env cd' r' cd r sfs)
   thus ?case 
-    by (induction "TCOS vs ((env, TCOPushLam cd' r' (length env) # cd, r) # sfs)" \<Sigma>'' 
-        rule: evaltco.induct) 
+    by (induction "TCOS vs ((env, TCOPushLam cd' r' # cd, r) # sfs)" \<Sigma>'' rule: evaltco.induct) 
        simp_all 
 next
   case (evtco_apply v env' cd' r' vs env cd r sfs)
@@ -57,13 +55,11 @@ next
        simp_all 
 next
   case (evtco_return vs env sfs)
-  thus ?case 
-    by (induction "TCOS vs ((env, [], TCOReturn (length env)) # sfs)" \<Sigma>'' rule: evaltco.induct)
-       simp_all 
+  thus ?case by (induction "TCOS vs ((env, [], TCOReturn) # sfs)" \<Sigma>'' rule: evaltco.induct) simp_all 
 next
   case (evtco_jump v env' cd' r' vs env sfs)
   thus ?case 
-    by (induction "TCOS (v # TCOLam env' cd' r' # vs) ((env, [], TCOJump (length env)) # sfs)" \<Sigma>''
+    by (induction "TCOS (v # TCOLam env' cd' r' # vs) ((env, [], TCOJump) # sfs)" \<Sigma>''
         rule: evaltco.induct) 
        simp_all 
 qed
