07TailCall/TailCallOptimization.thy
@@ -2,18 +2,18 @@ theory TailCallOptimization
   imports TailCall "../06TreeCode/TreeCode" "../00Utils/Iteration"
 begin
 
-fun tco_r :: "nat \<Rightarrow> tree_code list \<Rightarrow> tco_return" where
-  "tco_r d [] = TCOReturn d"
-| "tco_r d (TApply # cd) = (case cd of 
-      [] \<Rightarrow> TCOJump d
-    | _ \<Rightarrow> tco_r d cd)"
-| "tco_r d (op # cd) = tco_r d cd"
+fun tco_r :: "tree_code list \<Rightarrow> tco_return" where
+  "tco_r [] = TCOReturn"
+| "tco_r (TApply # cd) = (case cd of 
+      [] \<Rightarrow> TCOJump
+    | _ \<Rightarrow> tco_r cd)"
+| "tco_r (op # cd) = tco_r cd"
 
 fun tco_cd :: "tree_code list \<Rightarrow> tco_code list" where
   "tco_cd [] = []"
 | "tco_cd (TLookup x # cd) = TCOLookup x # tco_cd cd"
 | "tco_cd (TPushCon k # cd) = TCOPushCon k # tco_cd cd"
-| "tco_cd (TPushLam cd' d # cd) = TCOPushLam (tco_cd cd') (tco_r (Suc d) cd') d # tco_cd cd"
+| "tco_cd (TPushLam cd' # cd) = TCOPushLam (tco_cd cd') (tco_r cd') # tco_cd cd"
 | "tco_cd (TApply # cd) = (case cd of 
       [] \<Rightarrow> []
     | _ \<Rightarrow> TCOApply # tco_cd cd)"
@@ -21,22 +21,22 @@ fun tco_cd :: "tree_code list \<Rightarrow> tco_code list" where
 fun tco_cd_one :: "tree_code \<Rightarrow> tco_code" where
   "tco_cd_one (TLookup x) = TCOLookup x"
 | "tco_cd_one (TPushCon k) = TCOPushCon k"
-| "tco_cd_one (TPushLam cd' d) = TCOPushLam (tco_cd cd') (tco_r (Suc d) cd') d"
+| "tco_cd_one (TPushLam cd') = TCOPushLam (tco_cd cd') (tco_r cd')"
 | "tco_cd_one TApply = TCOApply"
 
 definition tco :: "tree_code list \<Rightarrow> tco_code list \<times> tco_return" where
-  "tco cd = (tco_cd cd, tco_r 0 cd)"
+  "tco cd = (tco_cd cd, tco_r cd)"
 
 primrec tco_val :: "tclosure \<Rightarrow> tco_closure" where
   "tco_val (TConst k) = TCOConst k"
-| "tco_val (TLam vs cd) = TCOLam (map tco_val vs) (tco_cd cd) (tco_r (Suc (length vs)) cd)"
+| "tco_val (TLam vs cd) = TCOLam (map tco_val vs) (tco_cd cd) (tco_r cd)"
 
 fun tco_stack_frame :: "tree_stack_frame \<Rightarrow> tco_stack_frame" where
-  "tco_stack_frame (vs, cd) = (map tco_val vs, tco_cd cd, tco_r (length vs) cd)"
+  "tco_stack_frame (vs, cd) = (map tco_val vs, tco_cd cd, tco_r cd)"
 
 fun live_frame :: "tco_stack_frame \<Rightarrow> bool" where
-  "live_frame (vs, [], TCOReturn d) = (d \<noteq> length vs)"
-| "live_frame (vs, [], TCOJump d) = True"
+  "live_frame (vs, [], TCOReturn) = False"
+| "live_frame (vs, [], TCOJump) = True"
 | "live_frame (vs, op # cd, r) = True"
 
 primrec dead_frame :: "tree_stack_frame \<Rightarrow> bool" where
@@ -48,10 +48,10 @@ abbreviation tco_stack :: "tree_stack_frame list \<Rightarrow> tco_stack_frame l
 primrec tco_state :: "tree_code_state \<Rightarrow> tco_code_state" where
   "tco_state (TS vs sfs) = TCOS (map tco_val vs) (tco_stack sfs)"
 
-lemma [simp]: "cd \<noteq> [] \<Longrightarrow> tco_r d (op # cd) = tco_r d cd"
+lemma [simp]: "cd \<noteq> [] \<Longrightarrow> tco_r (op # cd) = tco_r cd"
   by (induction op) (simp_all split: list.splits)
 
-lemma tco_r_append [simp]: "cd' \<noteq> [] \<Longrightarrow> tco_r d (cd @ cd') = tco_r d cd'"
+lemma tco_r_append [simp]: "cd' \<noteq> [] \<Longrightarrow> tco_r (cd @ cd') = tco_r cd'"
   by (induction cd) simp_all
 
 lemma [simp]: "cd \<noteq> [] \<Longrightarrow> tco_cd (op # cd) = tco_cd_one op # tco_cd cd"
@@ -65,7 +65,7 @@ lemma [simp]: "cd \<noteq> [] \<Longrightarrow> cd' \<noteq> [] \<Longrightarrow
 
 lemma [dest]: "(env, cd, r) # sfs = tco_stack sfs' \<Longrightarrow> \<exists>dsfs env' cd' sfs''. 
   sfs' = dsfs @ (env', cd') # sfs'' \<and> env = map tco_val env' \<and> cd = tco_cd cd' \<and> 
-    r = tco_r (length env) cd' \<and> list_all dead_frame dsfs \<and> sfs = tco_stack sfs''"
+    r = tco_r cd' \<and> list_all dead_frame dsfs \<and> sfs = tco_stack sfs''"
 proof (induction sfs')
   case (Cons sf sfs')
   thus ?case
@@ -75,8 +75,8 @@ proof (induction sfs')
     proof (induction cd' rule: tco_cd.induct)
       case 1
       then obtain dsfs env'' cd' sfs'' where X: "sfs' = dsfs @ (env'', cd') # sfs'' \<and> 
-        env = map tco_val env'' \<and> cd = tco_cd cd' \<and> r = tco_r (length env'') cd' \<and> 
-          list_all dead_frame dsfs \<and> sfs = tco_stack sfs''" by auto
+        env = map tco_val env'' \<and> cd = tco_cd cd' \<and> r = tco_r cd' \<and> list_all dead_frame dsfs \<and> 
+          sfs = tco_stack sfs''" by auto
       hence "\<exists>dsfsx. (env', []) # dsfs @ (env'', cd') # sfs'' = dsfsx @ (env'', cd') # sfs'' \<and> 
           list_all dead_frame dsfsx \<and> sfs = tco_stack sfs''" by simp
       hence "\<exists>dsfsx sfs'''. 
@@ -85,32 +85,31 @@ proof (induction sfs')
       with X show ?case by fastforce
     next
       case (2 x cd')
-      hence "env = map tco_val env' \<and> cd = TCOLookup x # tco_cd cd' \<and> r = tco_r (length env') cd' \<and> 
+      hence "env = map tco_val env' \<and> cd = TCOLookup x # tco_cd cd' \<and> r = tco_r cd' \<and> 
         sfs = tco_stack sfs'" by simp
       thus ?case by fastforce
     next
       case (3 k cd')
-      hence "env = map tco_val env' \<and> cd = TCOPushCon k # tco_cd cd' \<and> 
-        r = tco_r (length env') cd' \<and> sfs = tco_stack sfs'" by simp
+      hence "env = map tco_val env' \<and> cd = TCOPushCon k # tco_cd cd' \<and> r = tco_r cd' \<and> 
+        sfs = tco_stack sfs'" by simp
       thus ?case by fastforce
     next
-      case (4 cd\<^sub>l d cd')
-      hence "env = map tco_val env' \<and> 
-        cd = TCOPushLam (tco_cd cd\<^sub>l) (tco_r (Suc d) cd\<^sub>l) d # tco_cd cd' \<and> 
-          r = tco_r (length env') cd' \<and> sfs = tco_stack sfs'" by simp
+      case (4 cd\<^sub>l cd')
+      hence "env = map tco_val env' \<and> cd = TCOPushLam (tco_cd cd\<^sub>l) (tco_r cd\<^sub>l) # tco_cd cd' \<and> 
+        r = tco_r cd' \<and> sfs = tco_stack sfs'" by simp
       thus ?case by fastforce
     next
       case (5 cd')
       thus ?case
       proof (cases cd')
         case Nil
-        moreover with 5 have "env = map tco_val env' \<and> cd = [] \<and> r = TCOJump (length env') \<and> 
-          sfs = tco_stack sfs'" by simp
+        moreover with 5 have "env = map tco_val env' \<and> cd = [] \<and> r = TCOJump \<and> sfs = tco_stack sfs'" 
+          by simp
         ultimately show ?thesis by fastforce
       next
         case (Cons op cd'')
         moreover with 5 have "env = map tco_val env' \<and> cd = TCOApply # tco_cd (op # cd'') \<and> 
-          r = tco_r (length env') (op # cd'') \<and> sfs = tco_stack sfs'" by simp
+          r = tco_r (op # cd'') \<and> sfs = tco_stack sfs'" by simp
         ultimately show ?thesis by fastforce
       qed
     qed
@@ -119,7 +118,7 @@ qed simp_all
 
 lemma [dest]: "TCOS vs ((env, cd, r) # sfs) = tco_state \<Sigma> \<Longrightarrow> \<exists>dsfs vs' env' cd' sfs'. 
   \<Sigma> = TS vs' (dsfs @ (env', cd') # sfs') \<and> vs = map tco_val vs' \<and> env = map tco_val env' \<and> 
-    cd = tco_cd cd' \<and> r = tco_r (length env) cd' \<and> list_all dead_frame dsfs \<and> sfs = tco_stack sfs'"
+    cd = tco_cd cd' \<and> r = tco_r cd' \<and> list_all dead_frame dsfs \<and> sfs = tco_stack sfs'"
   by (induction \<Sigma>) auto
 
 lemma [dest]: "TCOLookup x # cd = tco_cd cd' \<Longrightarrow> \<exists>cd''. cd' = TLookup x # cd'' \<and> cd = tco_cd cd''"
@@ -128,9 +127,8 @@ lemma [dest]: "TCOLookup x # cd = tco_cd cd' \<Longrightarrow> \<exists>cd''. cd
 lemma [dest]: "TCOPushCon k # cd = tco_cd cd' \<Longrightarrow> \<exists>cd''. cd' = TPushCon k # cd'' \<and> cd = tco_cd cd''"
   by (induction cd' rule: tco_cd.induct) (simp_all split: list.splits)
 
-lemma [dest]: "TCOPushLam cd' r d # cd = tco_cd cd\<^sub>t \<Longrightarrow> 
-  \<exists>cd\<^sub>t' cd\<^sub>t''. cd\<^sub>t = TPushLam cd\<^sub>t'' d # cd\<^sub>t' \<and> cd = tco_cd cd\<^sub>t' \<and> r = tco_r (Suc d) cd\<^sub>t'' \<and> 
-    cd' = tco_cd cd\<^sub>t''"
+lemma [dest]: "TCOPushLam cd' r # cd = tco_cd cd\<^sub>t \<Longrightarrow> \<exists>cd\<^sub>t' cd\<^sub>t''. cd\<^sub>t = TPushLam cd\<^sub>t'' # cd\<^sub>t' \<and> 
+    cd = tco_cd cd\<^sub>t' \<and> r = tco_r cd\<^sub>t'' \<and> cd' = tco_cd cd\<^sub>t''"
   by (induction cd\<^sub>t rule: tco_cd.induct) (simp_all split: list.splits)
 
 lemma [dest]: "TCOApply # cd = tco_cd cd' \<Longrightarrow> 
@@ -141,14 +139,13 @@ lemma [dest]: "TCOConst k = tco_val v \<Longrightarrow> v = TConst k"
   by (induction v) simp_all
 
 lemma [dest]: "TCOLam env cd r = tco_val v \<Longrightarrow> 
-  \<exists>env\<^sub>t cd\<^sub>t. v = TLam env\<^sub>t cd\<^sub>t \<and> env = map tco_val env\<^sub>t \<and> cd = tco_cd cd\<^sub>t \<and> 
-    r = tco_r (Suc (length env\<^sub>t)) cd\<^sub>t"
+    \<exists>env\<^sub>t cd\<^sub>t. v = TLam env\<^sub>t cd\<^sub>t \<and> env = map tco_val env\<^sub>t \<and> cd = tco_cd cd\<^sub>t \<and> r = tco_r cd\<^sub>t"
   by (induction v) simp_all
 
-lemma [dest]: "TCOReturn d = tco_r d cd \<Longrightarrow> [] = tco_cd cd \<Longrightarrow> cd = []"
+lemma [dest]: "TCOReturn = tco_r cd \<Longrightarrow> [] = tco_cd cd \<Longrightarrow> cd = []"
   by (induction cd rule: tco_cd.induct) (simp_all split: list.splits)
 
-lemma [dest]: "TCOJump d = tco_r d cd \<Longrightarrow> [] = tco_cd cd \<Longrightarrow> cd = [TApply]"
+lemma [dest]: "TCOJump = tco_r cd \<Longrightarrow> [] = tco_cd cd \<Longrightarrow> cd = [TApply]"
   by (induction cd rule: tco_cd.induct) (simp_all split: list.splits)
 
 lemma [simp]: "list_all dead_frame dsfs \<Longrightarrow> iter (\<leadsto>\<^sub>t) (TS vs (dsfs @ sfs)) (TS vs sfs)"
@@ -161,22 +158,19 @@ qed simp_all
 
 lemma [simp]: "\<not> live_frame fr \<Longrightarrow> iter (\<leadsto>\<^sub>t\<^sub>c\<^sub>o) (TCOS vs (fr # sfs)) (TCOS vs sfs)"
 proof (induction fr rule: live_frame.induct)
-  case (1 env d)
-  hence "TCOS vs ((env, [], TCOReturn d) # sfs) \<leadsto>\<^sub>t\<^sub>c\<^sub>o TCOS vs sfs" by simp
-  thus ?case by simp
+  case (1 env)
+  hence "TCOS vs ((env, [], TCOReturn) # sfs) \<leadsto>\<^sub>t\<^sub>c\<^sub>o TCOS vs sfs" by simp
+  thus ?case by (metis iter_one)
 qed simp_all
 
-lemma [simp]: "tco_cd (op # cd) = [] \<Longrightarrow> tco_r d (op # cd) = TCOJump d"
+lemma [simp]: "tco_cd (op # cd) = [] \<Longrightarrow> tco_r (op # cd) = TCOJump"
   by (induction op) (simp_all split: list.splits)
 
-lemma [simp]: "live_frame (env, cd, TCOJump d)"
+lemma [simp]: "live_frame (env, cd, TCOJump)"
   by (induction cd) simp_all
 
-lemma [simp]: "live_frame (env, tco_cd (op # cd), tco_r d (op # cd))"
+lemma tco_never_dead [simp]: "live_frame (env, tco_cd (op # cd), tco_r (op # cd))"
   by (induction op) (simp_all split: list.splits)
-
-lemma tco_never_dead [simp]: "live_frame (vs, tco_cd (op # cd), tco_r (length vs) (op # cd))"
-  by (induction cd rule: tco_cd.induct) (simp_all split: list.splits)
 
 theorem completetco [simp]: "tco_state \<Sigma>\<^sub>t \<leadsto>\<^sub>t\<^sub>c\<^sub>o \<Sigma>' \<Longrightarrow> full_state \<Sigma>\<^sub>t \<Longrightarrow> \<exists>\<Sigma>\<^sub>t'. iter (\<leadsto>\<^sub>t) \<Sigma>\<^sub>t \<Sigma>\<^sub>t' \<and> 
   iter (\<leadsto>\<^sub>t\<^sub>c\<^sub>o) \<Sigma>' (tco_state \<Sigma>\<^sub>t')"
@@ -184,8 +178,8 @@ proof (induction "tco_state \<Sigma>\<^sub>t" \<Sigma>' rule: evaltco.induct)
   case (evtco_lookup env x v vs cd r sfs)
   then obtain dsfs vs' env' cd' sfs' where S: 
     "\<Sigma>\<^sub>t = TS vs' (dsfs @ (env', TLookup x # cd') # sfs') \<and> vs = map tco_val vs' \<and> 
-      env = map tco_val env' \<and> cd = tco_cd cd' \<and> r = tco_r (length env) cd' \<and> 
-        list_all dead_frame dsfs \<and> sfs = tco_stack sfs'" by fastforce
+      env = map tco_val env' \<and> cd = tco_cd cd' \<and> r = tco_r cd' \<and> list_all dead_frame dsfs \<and> 
+        sfs = tco_stack sfs'" by fastforce
   with evtco_lookup obtain v' where V: "lookup env' x = Some v' \<and> v = tco_val v'" by fastforce
   from S have "iter (\<leadsto>\<^sub>t) (TS vs' (dsfs @ (env', TLookup x # cd') # sfs')) 
     (TS vs' ((env', TLookup x # cd') # sfs'))" by simp
@@ -194,15 +188,15 @@ proof (induction "tco_state \<Sigma>\<^sub>t" \<Sigma>' rule: evaltco.induct)
   ultimately have X: "iter (\<leadsto>\<^sub>t) (TS vs' (dsfs @ (env', TLookup x # cd') # sfs')) 
     (TS (v' # vs') ((env', cd') # sfs'))" by (metis iter_append)
   from S V have "iter (\<leadsto>\<^sub>t\<^sub>c\<^sub>o) (TCOS (v # map tco_val vs') 
-    ((map tco_val env', tco_cd cd', tco_r (length env) cd') # tco_stack sfs')) 
+    ((map tco_val env', tco_cd cd', tco_r cd') # tco_stack sfs')) 
       (tco_state (TS (v' # vs') ((env', cd') # sfs')))" by simp
   with S X show ?case by blast
 next
   case (evtco_pushcon vs env k cd r sfs)
   then obtain dsfs vs' env' cd' sfs' where S: 
     "\<Sigma>\<^sub>t = TS vs' (dsfs @ (env', TPushCon k # cd') # sfs') \<and> vs = map tco_val vs' \<and> 
-      env = map tco_val env' \<and> cd = tco_cd cd' \<and> r = tco_r (length env) cd' \<and> 
-        list_all dead_frame dsfs \<and> sfs = tco_stack sfs'" by fastforce
+      env = map tco_val env' \<and> cd = tco_cd cd' \<and> r = tco_r cd' \<and> list_all dead_frame dsfs \<and> 
+        sfs = tco_stack sfs'" by fastforce
   hence "iter (\<leadsto>\<^sub>t) (TS vs' (dsfs @ (env', TPushCon k # cd') # sfs')) 
     (TS vs' ((env', TPushCon k # cd') # sfs'))" by simp
   moreover have "iter (\<leadsto>\<^sub>t) (TS vs' ((env', TPushCon k # cd') # sfs')) 
@@ -210,24 +204,23 @@ next
   ultimately have X: "iter (\<leadsto>\<^sub>t) (TS vs' (dsfs @ (env', TPushCon k # cd') # sfs')) 
     (TS (TConst k # vs') ((env', cd') # sfs'))" by simp
   from S have "iter (\<leadsto>\<^sub>t\<^sub>c\<^sub>o) (TCOS (TCOConst k # map tco_val vs') 
-    ((map tco_val env', tco_cd cd', tco_r (length env) cd') # tco_stack sfs')) 
+    ((map tco_val env', tco_cd cd', tco_r cd') # tco_stack sfs')) 
       (tco_state (TS (TConst k # vs') ((env', cd') # sfs')))" by simp
   with S X show ?case by blast
 next
   case (evtco_pushlam vs env cd' r' cd r sfs)
   then obtain dsfs vs\<^sub>t env\<^sub>t cd\<^sub>t cd\<^sub>t' sfs\<^sub>t where S: 
-    "\<Sigma>\<^sub>t = TS vs\<^sub>t (dsfs @ (env\<^sub>t, TPushLam cd\<^sub>t' (length env) # cd\<^sub>t) # sfs\<^sub>t) \<and> vs = map tco_val vs\<^sub>t \<and> 
-      env = map tco_val env\<^sub>t \<and> cd = tco_cd cd\<^sub>t \<and> cd' = tco_cd cd\<^sub>t' \<and> 
-        r' = tco_r (Suc (length env)) cd\<^sub>t' \<and> r = tco_r (length env) cd\<^sub>t \<and> list_all dead_frame dsfs \<and> 
-          sfs = tco_stack sfs\<^sub>t" by fastforce
-  hence "iter (\<leadsto>\<^sub>t) (TS vs\<^sub>t (dsfs @ (env\<^sub>t, TPushLam cd\<^sub>t' (length env) # cd\<^sub>t) # sfs\<^sub>t)) 
-    (TS vs\<^sub>t ((env\<^sub>t, TPushLam cd\<^sub>t' (length env\<^sub>t) # cd\<^sub>t) # sfs\<^sub>t))" by simp
-  moreover have "iter (\<leadsto>\<^sub>t) (TS vs\<^sub>t ((env\<^sub>t, TPushLam cd\<^sub>t' (length env\<^sub>t) # cd\<^sub>t) # sfs\<^sub>t)) 
+    "\<Sigma>\<^sub>t = TS vs\<^sub>t (dsfs @ (env\<^sub>t, TPushLam cd\<^sub>t' # cd\<^sub>t) # sfs\<^sub>t) \<and> vs = map tco_val vs\<^sub>t \<and> 
+      env = map tco_val env\<^sub>t \<and> cd = tco_cd cd\<^sub>t \<and> cd' = tco_cd cd\<^sub>t' \<and> r' = tco_r cd\<^sub>t' \<and> 
+        r = tco_r cd\<^sub>t \<and> list_all dead_frame dsfs \<and> sfs = tco_stack sfs\<^sub>t" by fastforce
+  hence "iter (\<leadsto>\<^sub>t) (TS vs\<^sub>t (dsfs @ (env\<^sub>t, TPushLam cd\<^sub>t' # cd\<^sub>t) # sfs\<^sub>t)) 
+    (TS vs\<^sub>t ((env\<^sub>t, TPushLam cd\<^sub>t' # cd\<^sub>t) # sfs\<^sub>t))" by simp
+  moreover have "iter (\<leadsto>\<^sub>t) (TS vs\<^sub>t ((env\<^sub>t, TPushLam cd\<^sub>t' # cd\<^sub>t) # sfs\<^sub>t)) 
     (TS (TLam env\<^sub>t cd\<^sub>t' # vs\<^sub>t) ((env\<^sub>t, cd\<^sub>t) # sfs\<^sub>t))" by (metis evt_pushlam iter_one)
-  ultimately have X: "iter (\<leadsto>\<^sub>t) (TS vs\<^sub>t (dsfs @ (env\<^sub>t, TPushLam cd\<^sub>t' (length env) # cd\<^sub>t) # sfs\<^sub>t)) 
+  ultimately have X: "iter (\<leadsto>\<^sub>t) (TS vs\<^sub>t (dsfs @ (env\<^sub>t, TPushLam cd\<^sub>t' # cd\<^sub>t) # sfs\<^sub>t)) 
     (TS (TLam env\<^sub>t cd\<^sub>t' # vs\<^sub>t) ((env\<^sub>t, cd\<^sub>t) # sfs\<^sub>t))" by simp
   from S have "iter (\<leadsto>\<^sub>t\<^sub>c\<^sub>o) (TCOS (TCOLam env cd' r' # map tco_val vs\<^sub>t) 
-    ((map tco_val env\<^sub>t, tco_cd cd\<^sub>t, tco_r (length env) cd\<^sub>t) # tco_stack sfs\<^sub>t)) 
+    ((map tco_val env\<^sub>t, tco_cd cd\<^sub>t, tco_r cd\<^sub>t) # tco_stack sfs\<^sub>t)) 
       (tco_state (TS (TLam env\<^sub>t cd\<^sub>t' # vs\<^sub>t) ((env\<^sub>t, cd\<^sub>t) # sfs\<^sub>t)))" by simp
   with S X show ?case by blast
 next
@@ -235,11 +228,11 @@ next
   then obtain dsfs v\<^sub>t vl vs\<^sub>t env\<^sub>t cd\<^sub>t'' sfs\<^sub>t where S: 
     "\<Sigma>\<^sub>t = TS (v\<^sub>t # vl # vs\<^sub>t) (dsfs @ (env\<^sub>t, cd\<^sub>t'') # sfs\<^sub>t) \<and> v = tco_val v\<^sub>t \<and> 
       TCOLam env' cd' r' = tco_val vl \<and> vs = map tco_val vs\<^sub>t \<and> env = map tco_val env\<^sub>t \<and> 
-        TCOApply # cd = tco_cd cd\<^sub>t'' \<and> r = tco_r (length env) cd\<^sub>t'' \<and> list_all dead_frame dsfs \<and> 
+        TCOApply # cd = tco_cd cd\<^sub>t'' \<and> r = tco_r cd\<^sub>t'' \<and> list_all dead_frame dsfs \<and> 
           sfs = tco_stack sfs\<^sub>t" by blast
   then obtain op cd\<^sub>t where C: "cd\<^sub>t'' = TApply # op # cd\<^sub>t \<and> cd = tco_cd (op # cd\<^sub>t)" by blast
   from S obtain env\<^sub>t' cd\<^sub>t' where V: "vl = TLam env\<^sub>t' cd\<^sub>t' \<and> env' = map tco_val env\<^sub>t' \<and> 
-    cd' = tco_cd cd\<^sub>t' \<and> r' = tco_r (Suc (length env\<^sub>t')) cd\<^sub>t'" by blast
+    cd' = tco_cd cd\<^sub>t' \<and> r' = tco_r cd\<^sub>t'" by blast
   from S have "iter (\<leadsto>\<^sub>t) (TS (v\<^sub>t # TLam env\<^sub>t' cd\<^sub>t' # vs\<^sub>t) (dsfs @ (env\<^sub>t, TApply # op # cd\<^sub>t) # sfs\<^sub>t)) 
     (TS (v\<^sub>t # TLam env\<^sub>t' cd\<^sub>t' # vs\<^sub>t) ((env\<^sub>t, TApply # op # cd\<^sub>t) # sfs\<^sub>t))" by simp
   moreover have "TS (v\<^sub>t # TLam env\<^sub>t' cd\<^sub>t' # vs\<^sub>t) ((env\<^sub>t, TApply # op # cd\<^sub>t) # sfs\<^sub>t) \<leadsto>\<^sub>t 
@@ -248,12 +241,11 @@ next
     (dsfs @ (env\<^sub>t, TApply # op # cd\<^sub>t) # sfs\<^sub>t)) (TS vs\<^sub>t ((v\<^sub>t # env\<^sub>t', cd\<^sub>t') # (env\<^sub>t, op # cd\<^sub>t) # sfs\<^sub>t))" 
       by simp
   from evtco_apply S V have "full_block cd\<^sub>t' 0 = Some (Suc 0)" by simp
-  hence "live_frame (tco_val v\<^sub>t # map tco_val env\<^sub>t', tco_cd cd\<^sub>t', tco_r (Suc (length env\<^sub>t')) cd\<^sub>t')" 
+  hence "live_frame (tco_val v\<^sub>t # map tco_val env\<^sub>t', tco_cd cd\<^sub>t', tco_r cd\<^sub>t')" 
     by (induction cd\<^sub>t' rule: tco_cd.induct) (simp_all split: list.splits)
   with S have "iter (\<leadsto>\<^sub>t\<^sub>c\<^sub>o) (TCOS (map tco_val vs\<^sub>t) ((tco_val v\<^sub>t # map tco_val env\<^sub>t', tco_cd cd\<^sub>t', 
-    tco_r (Suc (length env\<^sub>t')) cd\<^sub>t') # (map tco_val env\<^sub>t, tco_cd (op # cd\<^sub>t), 
-      tco_r (length env) (TApply # op # cd\<^sub>t)) # tco_stack sfs\<^sub>t)) 
-        (tco_state (TS vs\<^sub>t ((v\<^sub>t # env\<^sub>t', cd\<^sub>t') # (env\<^sub>t, op # cd\<^sub>t) # sfs\<^sub>t)))" by simp
+    tco_r cd\<^sub>t') # (map tco_val env\<^sub>t, tco_cd (op # cd\<^sub>t), tco_r (TApply # op # cd\<^sub>t)) # tco_stack sfs\<^sub>t)) 
+      (tco_state (TS vs\<^sub>t ((v\<^sub>t # env\<^sub>t', cd\<^sub>t') # (env\<^sub>t, op # cd\<^sub>t) # sfs\<^sub>t)))" by simp
   with S C V X show ?case by blast
 next
   case (evtco_return vs env sfs)
@@ -270,10 +262,10 @@ next
   then obtain dsfs v\<^sub>t vl vs\<^sub>t env\<^sub>t cd\<^sub>t sfs\<^sub>t where S: 
     "\<Sigma>\<^sub>t = TS (v\<^sub>t # vl # vs\<^sub>t) (dsfs @ (env\<^sub>t, cd\<^sub>t) # sfs\<^sub>t) \<and> v = tco_val v\<^sub>t \<and> 
       TCOLam env' cd' r' = tco_val vl \<and> vs = map tco_val vs\<^sub>t \<and> env = map tco_val env\<^sub>t \<and> 
-        [] = tco_cd cd\<^sub>t \<and> TCOJump (length env) = tco_r (length env) cd\<^sub>t \<and> list_all dead_frame dsfs \<and> 
+        [] = tco_cd cd\<^sub>t \<and> TCOJump = tco_r cd\<^sub>t \<and> list_all dead_frame dsfs \<and> 
           sfs = tco_stack sfs\<^sub>t" by blast
   then obtain env\<^sub>t' cd\<^sub>t' where V: "vl = TLam env\<^sub>t' cd\<^sub>t' \<and> env' = map tco_val env\<^sub>t' \<and> 
-    cd' = tco_cd cd\<^sub>t' \<and> r' = tco_r (Suc (length env\<^sub>t')) cd\<^sub>t'" by blast
+    cd' = tco_cd cd\<^sub>t' \<and> r' = tco_r cd\<^sub>t'" by blast
   from S have C: "cd\<^sub>t = [TApply]" by blast
   with S have "iter (\<leadsto>\<^sub>t) (TS (v\<^sub>t # TLam env\<^sub>t' cd\<^sub>t' # vs\<^sub>t) (dsfs @ (env\<^sub>t, [TApply]) # sfs\<^sub>t)) 
     (TS (v\<^sub>t # TLam env\<^sub>t' cd\<^sub>t' # vs\<^sub>t) ((env\<^sub>t, [TApply]) # sfs\<^sub>t))" by simp
@@ -281,9 +273,8 @@ next
     (TS vs\<^sub>t ((v\<^sub>t # env\<^sub>t', cd\<^sub>t') # (env\<^sub>t, []) # sfs\<^sub>t))" by (simp add: iter_one)
   ultimately have X: "iter (\<leadsto>\<^sub>t) (TS (v\<^sub>t # TLam env\<^sub>t' cd\<^sub>t' # vs\<^sub>t) (dsfs @ (env\<^sub>t, [TApply]) # sfs\<^sub>t)) 
     (TS vs\<^sub>t ((v\<^sub>t # env\<^sub>t', cd\<^sub>t') # (env\<^sub>t, []) # sfs\<^sub>t))" using iter_append by fastforce
-  have "iter (\<leadsto>\<^sub>t\<^sub>c\<^sub>o) (TCOS (map tco_val vs\<^sub>t) 
-    ((tco_val v\<^sub>t # map tco_val env\<^sub>t', tco_cd cd\<^sub>t', tco_r (Suc (length env\<^sub>t')) cd\<^sub>t') # tco_stack sfs\<^sub>t)) 
-      (tco_state (TS vs\<^sub>t ((v\<^sub>t # env\<^sub>t', cd\<^sub>t') # (env\<^sub>t, []) # sfs\<^sub>t)))" by simp
+  have "iter (\<leadsto>\<^sub>t\<^sub>c\<^sub>o) (TCOS (map tco_val vs\<^sub>t) ((tco_val v\<^sub>t # map tco_val env\<^sub>t', tco_cd cd\<^sub>t', tco_r cd\<^sub>t') 
+    # tco_stack sfs\<^sub>t)) (tco_state (TS vs\<^sub>t ((v\<^sub>t # env\<^sub>t', cd\<^sub>t') # (env\<^sub>t, []) # sfs\<^sub>t)))" by simp
   with S V C X show ?case by blast
 qed
 
@@ -293,15 +284,12 @@ proof (induction \<Sigma> \<Sigma>' rule: evalt.induct)
   thus ?case 
   proof (cases cd)
     case Nil
-    have "TCOS (tco_val v # map tco_val vs) 
-      ((map tco_val env, [], TCOReturn (length env)) # tco_stack sfs) \<leadsto>\<^sub>t\<^sub>c\<^sub>o 
-        TCOS (tco_val v # map tco_val vs) (tco_stack sfs)" by (metis evtco_return length_map)
-    hence "TCOS (tco_val v # map tco_val vs) 
-      ((map tco_val env, [], TCOReturn (length env)) # tco_stack sfs) \<leadsto>\<^sub>t\<^sub>c\<^sub>o 
-        tco_state (TS (v # vs) ((env, []) # sfs))" by simp
+    have "TCOS (tco_val v # map tco_val vs) ((map tco_val env, [], TCOReturn) # tco_stack sfs) \<leadsto>\<^sub>t\<^sub>c\<^sub>o 
+      TCOS (tco_val v # map tco_val vs) (tco_stack sfs)" by (metis evtco_return)
+    hence "TCOS (tco_val v # map tco_val vs) ((map tco_val env, [], TCOReturn) # tco_stack sfs) \<leadsto>\<^sub>t\<^sub>c\<^sub>o 
+      tco_state (TS (v # vs) ((env, []) # sfs))" by simp
     moreover from evt_lookup have "tco_state (TS vs ((env, [TLookup x]) # sfs)) \<leadsto>\<^sub>t\<^sub>c\<^sub>o
-      TCOS (tco_val v # map tco_val vs) 
-        ((map tco_val env, [], TCOReturn (length env)) # tco_stack sfs)" by simp
+      TCOS (tco_val v # map tco_val vs) ((map tco_val env, [], TCOReturn) # tco_stack sfs)" by simp
     ultimately have "iter (\<leadsto>\<^sub>t\<^sub>c\<^sub>o) (tco_state (TS vs ((env, [TLookup x]) # sfs)))
       (tco_state (TS (v # vs) ((env, []) # sfs)))" by (metis iter_refl iter_step)
     with Nil show ?thesis by simp
@@ -316,15 +304,14 @@ next
   thus ?case 
   proof (cases cd)
     case Nil
-    have "TCOS (TCOConst k # map tco_val vs) 
-      ((map tco_val env, [], TCOReturn (length env)) # tco_stack sfs) \<leadsto>\<^sub>t\<^sub>c\<^sub>o 
-        TCOS (TCOConst k # map tco_val vs) (tco_stack sfs)" by (metis evtco_return length_map)
+    have "TCOS (TCOConst k # map tco_val vs) ((map tco_val env, [], TCOReturn) # tco_stack sfs) \<leadsto>\<^sub>t\<^sub>c\<^sub>o 
+        TCOS (TCOConst k # map tco_val vs) (tco_stack sfs)" by (metis evtco_return)
     hence "TCOS (TCOConst k # map tco_val vs) 
-      ((map tco_val env, [], TCOReturn (length env)) # tco_stack sfs) \<leadsto>\<^sub>t\<^sub>c\<^sub>o 
+      ((map tco_val env, [], TCOReturn) # tco_stack sfs) \<leadsto>\<^sub>t\<^sub>c\<^sub>o 
         tco_state (TS (TConst k # vs) ((env, []) # sfs))" by simp
     moreover have "tco_state (TS vs ((env, [TPushCon k]) # sfs)) \<leadsto>\<^sub>t\<^sub>c\<^sub>o
       TCOS (TCOConst k # map tco_val vs) 
-        ((map tco_val env, [], TCOReturn (length env)) # tco_stack sfs)" by simp
+        ((map tco_val env, [], TCOReturn) # tco_stack sfs)" by simp
     ultimately have "iter (\<leadsto>\<^sub>t\<^sub>c\<^sub>o) (tco_state (TS vs ((env, [TPushCon k]) # sfs)))
       (tco_state (TS (TConst k # vs) ((env, []) # sfs)))" by (metis iter_refl iter_step)
     with Nil show ?thesis by simp
@@ -340,36 +327,31 @@ next
   proof (cases cd)
     case Nil
     have "TCOS (map tco_val vs) ((map tco_val env, 
-      [TCOPushLam (tco_cd cd') (tco_r (Suc (length env)) cd') (length env)], 
-        TCOReturn (length env)) # tco_stack sfs) \<leadsto>\<^sub>t\<^sub>c\<^sub>o  TCOS (TCOLam (map tco_val env) (tco_cd cd') 
-          (tco_r (Suc (length env)) cd') # map tco_val vs)
-            ((map tco_val env, [], TCOReturn (length env)) # tco_stack sfs)" 
-      by (metis evtco_pushlam length_map)
-    hence X: "tco_state (TS vs ((env, [TPushLam cd' (length env)]) # sfs)) \<leadsto>\<^sub>t\<^sub>c\<^sub>o
-      TCOS (TCOLam (map tco_val env) (tco_cd cd') (tco_r (Suc (length env)) cd') # map tco_val vs) 
-        ((map tco_val env, [], TCOReturn (length env)) # tco_stack sfs)" by simp
-    have "TCOS (TCOLam (map tco_val env) (tco_cd cd') (tco_r (Suc (length env)) cd') # 
-      map tco_val vs) ((map tco_val env, [], TCOReturn (length env)) # tco_stack sfs) \<leadsto>\<^sub>t\<^sub>c\<^sub>o
-        TCOS (TCOLam (map tco_val env) (tco_cd cd') (tco_r (Suc (length env)) cd') # map tco_val vs) 
-          (tco_stack sfs)" by (metis evtco_return length_map)
-    hence "TCOS (TCOLam (map tco_val env) (tco_cd cd') (tco_r (Suc (length env)) cd') # 
-      map tco_val vs) ((map tco_val env, [], TCOReturn (length env)) # tco_stack sfs) \<leadsto>\<^sub>t\<^sub>c\<^sub>o
+      [TCOPushLam (tco_cd cd') (tco_r cd')], TCOReturn) # tco_stack sfs) \<leadsto>\<^sub>t\<^sub>c\<^sub>o  
+        TCOS (TCOLam (map tco_val env) (tco_cd cd') (tco_r cd') # map tco_val vs) 
+          ((map tco_val env, [], TCOReturn) # tco_stack sfs)" by (metis evtco_pushlam)
+    hence X: "tco_state (TS vs ((env, [TPushLam cd']) # sfs)) \<leadsto>\<^sub>t\<^sub>c\<^sub>o
+      TCOS (TCOLam (map tco_val env) (tco_cd cd') (tco_r cd') # map tco_val vs) 
+        ((map tco_val env, [], TCOReturn) # tco_stack sfs)" by simp
+    have "TCOS (TCOLam (map tco_val env) (tco_cd cd') (tco_r cd') # 
+      map tco_val vs) ((map tco_val env, [], TCOReturn) # tco_stack sfs) \<leadsto>\<^sub>t\<^sub>c\<^sub>o
+        TCOS (TCOLam (map tco_val env) (tco_cd cd') (tco_r cd') # map tco_val vs) (tco_stack sfs)" 
+          by (metis evtco_return)
+    hence "TCOS (TCOLam (map tco_val env) (tco_cd cd') (tco_r cd') # 
+      map tco_val vs) ((map tco_val env, [], TCOReturn) # tco_stack sfs) \<leadsto>\<^sub>t\<^sub>c\<^sub>o
         tco_state (TS (TLam env cd' # vs) ((env, []) # sfs))" by simp
-    with X have "iter (\<leadsto>\<^sub>t\<^sub>c\<^sub>o) (tco_state (TS vs ((env, [TPushLam cd' (length env)]) # sfs)))
+    with X have "iter (\<leadsto>\<^sub>t\<^sub>c\<^sub>o) (tco_state (TS vs ((env, [TPushLam cd']) # sfs)))
       (tco_state (TS (TLam env cd' # vs) ((env, []) # sfs)))" by (metis iter_refl iter_step)
     with Nil show ?thesis by simp
   next
     case (Cons op cd)
-    have "TCOS (map tco_val vs) ((map tco_val env, 
-      TCOPushLam (tco_cd cd') (tco_r (Suc (length env)) cd') (length env) # tco_cd (op # cd), 
-        tco_r (length env) (op # cd)) # tco_stack sfs) \<leadsto>\<^sub>t\<^sub>c\<^sub>o
-          TCOS (TCOLam (map tco_val env) (tco_cd cd') (tco_r (Suc (length env)) cd') # 
-            map tco_val vs) ((map tco_val env, tco_cd (op # cd), tco_r (length env) (op # cd)) # 
-              tco_stack sfs)" 
-      by (metis evtco_pushlam length_map)
-    hence 
-      "tco_state (TS vs ((env, TPushLam cd' (length env) # op # cd) # sfs)) \<leadsto>\<^sub>t\<^sub>c\<^sub>o
-        tco_state (TS (TLam env cd' # vs) ((env, op # cd) # sfs))" by simp
+    have "TCOS (map tco_val vs) ((map tco_val env, TCOPushLam (tco_cd cd') (tco_r cd') # 
+      tco_cd (op # cd), tco_r (op # cd)) # tco_stack sfs) \<leadsto>\<^sub>t\<^sub>c\<^sub>o
+        TCOS (TCOLam (map tco_val env) (tco_cd cd') (tco_r cd') # map tco_val vs) 
+          ((map tco_val env, tco_cd (op # cd), tco_r (op # cd)) # tco_stack sfs)" 
+      by (metis evtco_pushlam)
+    hence "tco_state (TS vs ((env, TPushLam cd' # op # cd) # sfs)) \<leadsto>\<^sub>t\<^sub>c\<^sub>o
+      tco_state (TS (TLam env cd' # vs) ((env, op # cd) # sfs))" by simp
     with Cons show ?thesis by (metis iter_one)
   qed
 next
@@ -380,33 +362,28 @@ next
     thus ?thesis
     proof (cases cd')
       case Nil
-      have "TCOS (map tco_val vs) ((tco_val v # map tco_val env', [], 
-        TCOReturn (length (tco_val v # map tco_val env'))) # tco_stack sfs) \<leadsto>\<^sub>t\<^sub>c\<^sub>o
-          TCOS (map tco_val vs) (tco_stack sfs)" by (metis evtco_return)
-      hence "TCOS (map tco_val vs) ((tco_val v # map tco_val env', [], 
-        TCOReturn (Suc (length env'))) # tco_stack sfs) \<leadsto>\<^sub>t\<^sub>c\<^sub>o 
-          tco_state (TS vs ((v # env', []) # (env, []) # sfs))" by simp
-      hence X: "iter (\<leadsto>\<^sub>t\<^sub>c\<^sub>o) (TCOS (map tco_val vs) 
-        ((tco_val v # map tco_val env', [], TCOReturn (Suc (length env'))) # tco_stack sfs))
-          (tco_state (TS vs ((v # env', []) # (env, []) # sfs)))" by (metis iter_one)
-      have "TCOS (tco_val v # TCOLam (map tco_val env') [] (TCOReturn (Suc (length env'))) # 
-        map tco_val vs) ((map tco_val env, [], TCOJump (length env)) # tco_stack sfs) \<leadsto>\<^sub>t\<^sub>c\<^sub>o
-          TCOS (map tco_val vs) ((tco_val v # map tco_val env', [], TCOReturn (Suc (length env'))) # 
-            tco_stack sfs)" by (metis evtco_jump length_map)
+      have "TCOS (map tco_val vs) ((tco_val v # map tco_val env', [], TCOReturn) # tco_stack sfs) 
+        \<leadsto>\<^sub>t\<^sub>c\<^sub>o TCOS (map tco_val vs) (tco_stack sfs)" by (metis evtco_return)
+      hence "TCOS (map tco_val vs) ((tco_val v # map tco_val env', [], TCOReturn) # tco_stack sfs) 
+        \<leadsto>\<^sub>t\<^sub>c\<^sub>o tco_state (TS vs ((v # env', []) # (env, []) # sfs))" by simp
+      hence X: "iter (\<leadsto>\<^sub>t\<^sub>c\<^sub>o) (TCOS (map tco_val vs) ((tco_val v # map tco_val env', [], TCOReturn) # 
+        tco_stack sfs)) (tco_state (TS vs ((v # env', []) # (env, []) # sfs)))" by (metis iter_one)
+      have "TCOS (tco_val v # TCOLam (map tco_val env') [] TCOReturn # 
+        map tco_val vs) ((map tco_val env, [], TCOJump) # tco_stack sfs) \<leadsto>\<^sub>t\<^sub>c\<^sub>o
+          TCOS (map tco_val vs) ((tco_val v # map tco_val env', [], TCOReturn) # 
+            tco_stack sfs)" by (metis evtco_jump)
       hence "tco_state (TS (v # TLam env' [] # vs) ((env, [TApply]) # sfs)) \<leadsto>\<^sub>t\<^sub>c\<^sub>o
-        TCOS (map tco_val vs) ((tco_val v # map tco_val env', [], TCOReturn (Suc (length env'))) # 
-          tco_stack sfs)" by simp
+        TCOS (map tco_val vs) ((tco_val v # map tco_val env', [], TCOReturn) # tco_stack sfs)" 
+          by simp
       with X have "iter (\<leadsto>\<^sub>t\<^sub>c\<^sub>o) (tco_state (TS (v # TLam env' [] # vs) ((env, [TApply]) # sfs)))
         (tco_state (TS vs ((v # env', []) # (env, []) # sfs)))" using iter_step by fast
       with CD Nil show ?thesis by simp
     next
       case (Cons op' cd'')
-      have "TCOS (tco_val v # TCOLam (map tco_val env') (tco_cd (op' # cd'')) 
-        (tco_r (Suc (length env')) (op' # cd'')) # map tco_val vs) 
-          ((map tco_val env, [], TCOJump (length env)) # tco_stack sfs) \<leadsto>\<^sub>t\<^sub>c\<^sub>o
-            TCOS (map tco_val vs) ((tco_val v # map tco_val env', tco_cd (op' # cd''), 
-              tco_r (Suc (length env')) (op' # cd'')) # tco_stack sfs)" 
-        by (metis evtco_jump length_map)
+      have "TCOS (tco_val v # TCOLam (map tco_val env') (tco_cd (op' # cd'')) (tco_r (op' # cd'')) # 
+        map tco_val vs) ((map tco_val env, [], TCOJump) # tco_stack sfs) \<leadsto>\<^sub>t\<^sub>c\<^sub>o
+          TCOS (map tco_val vs) ((tco_val v # map tco_val env', tco_cd (op' # cd''), 
+            tco_r (op' # cd'')) # tco_stack sfs)"  by (metis evtco_jump)
       hence "tco_state (TS (v # TLam env' (op' # cd'') # vs) ((env, [TApply]) # sfs)) \<leadsto>\<^sub>t\<^sub>c\<^sub>o
         tco_state (TS vs ((v # env', op' # cd'') # (env, []) # sfs))" by simp
       with Nil Cons show ?thesis by (metis iter_one)
@@ -416,23 +393,19 @@ next
     thus ?thesis
     proof (cases cd')
       case Nil
-      have "TCOS (map tco_val vs) ((tco_val v # map tco_val env', [], 
-        TCOReturn (length (tco_val v # map tco_val env'))) # (map tco_val env, tco_cd (op # cd),
-          tco_r (length env) (op # cd)) # tco_stack sfs) \<leadsto>\<^sub>t\<^sub>c\<^sub>o
-            TCOS (map tco_val vs) ((map tco_val env, tco_cd (op # cd), 
-              tco_r (length env) (op # cd)) # tco_stack sfs)" by (metis evtco_return)
-      hence "TCOS (map tco_val vs) ((tco_val v # map tco_val env', [], 
-        TCOReturn (Suc (length env'))) # (map tco_val env, tco_cd (op # cd), 
-          tco_r (length env) (op # cd)) # tco_stack sfs) \<leadsto>\<^sub>t\<^sub>c\<^sub>o
+      have "TCOS (map tco_val vs) ((tco_val v # map tco_val env', [], TCOReturn) # 
+        (map tco_val env, tco_cd (op # cd), tco_r (op # cd)) # tco_stack sfs) \<leadsto>\<^sub>t\<^sub>c\<^sub>o
+          TCOS (map tco_val vs) ((map tco_val env, tco_cd (op # cd), 
+            tco_r (op # cd)) # tco_stack sfs)" by (metis evtco_return)
+      hence "TCOS (map tco_val vs) ((tco_val v # map tco_val env', [], TCOReturn) # 
+        (map tco_val env, tco_cd (op # cd), tco_r (op # cd)) # tco_stack sfs) \<leadsto>\<^sub>t\<^sub>c\<^sub>o
             tco_state (TS vs ((v # env', []) # (env, op # cd) # sfs))" by simp
-      hence X: "iter (\<leadsto>\<^sub>t\<^sub>c\<^sub>o) (TCOS (map tco_val vs) ((tco_val v # map tco_val env', [], 
-        TCOReturn (Suc (length env'))) # (map tco_val env, tco_cd (op # cd), 
-          tco_r (length env) (op # cd)) # tco_stack sfs)) 
-            (tco_state (TS vs ((v # env', []) # (env, op # cd) # sfs)))" by (metis iter_one)
+      hence X: "iter (\<leadsto>\<^sub>t\<^sub>c\<^sub>o) (TCOS (map tco_val vs) ((tco_val v # map tco_val env', [], TCOReturn) # 
+        (map tco_val env, tco_cd (op # cd), tco_r (op # cd)) # tco_stack sfs)) 
+          (tco_state (TS vs ((v # env', []) # (env, op # cd) # sfs)))" by (metis iter_one)
       have "tco_state (TS (v # TLam env' [] # vs) ((env, TApply # op # cd) # sfs)) \<leadsto>\<^sub>t\<^sub>c\<^sub>o
-        TCOS (map tco_val vs) ((tco_val v # map tco_val env', [], TCOReturn (Suc (length env'))) # 
-          (map tco_val env, tco_cd (op # cd), tco_r (length env) (op # cd)) # tco_stack sfs)" 
-            by simp
+        TCOS (map tco_val vs) ((tco_val v # map tco_val env', [], TCOReturn) # 
+          (map tco_val env, tco_cd (op # cd), tco_r (op # cd)) # tco_stack sfs)" by simp
       with X have "iter (\<leadsto>\<^sub>t\<^sub>c\<^sub>o) (tco_state (TS (v # TLam env' [] # vs) 
         ((env, TApply # op # cd) # sfs)))
           (tco_state (TS vs ((v # env', []) # (env, op # cd) # sfs)))" 
